UTP/ITree_UTP.thy
@@ -8,8 +8,9 @@ theory ITree_UTP
     ITree_Circus
     ITree_Relation
     ITree_Procedure
-    ITree_Hoare
     ITree_WP
+    ITree_Hoare
+    ITree_THoare
     ITree_DFP
     ITree_Designs
 begin end
